PiCore_IFS.thy
@@ -19,15 +19,15 @@ locale InfoFlow = event ptran petran fin_com
     and vpeq ::  "'s \<Rightarrow> 'd \<Rightarrow> 's \<Rightarrow> bool" ("(_ \<sim>_\<sim> _)" [70,69,70] 60)
     and obs ::  "'s \<Rightarrow> 'd \<Rightarrow> 'o" (infixl "\<guillemotright>"  55)
     and dome :: "'s  \<Rightarrow> ('l,'k,'s, 'prog) event \<Rightarrow> 'd"
-  assumes vpeq_transitive : "\<forall> a b c u. (a \<sim> u \<sim> b) \<and> (b \<sim> u \<sim> c) \<longrightarrow> (a \<sim> u \<sim> c)"
-    and   vpeq_symmetric : "\<forall> a b u. (a \<sim> u \<sim> b) \<longrightarrow> (b \<sim> u \<sim> a)"
-    and   vpeq_reflexive : "\<forall> a u. (a \<sim> u \<sim> a)"
-    and   step_def : "step a \<equiv> {(P, Q). (\<Gamma> \<turnstile> P -pes-(actk a)\<rightarrow> Q) \<and> 
+  assumes info_vpeq_trans : "\<forall> a b c u. (a \<sim> u \<sim> b) \<and> (b \<sim> u \<sim> c) \<longrightarrow> (a \<sim> u \<sim> c)"
+    and   info_vpeq_sym : "\<forall> a b u. (a \<sim> u \<sim> b) \<longrightarrow> (b \<sim> u \<sim> a)"
+    and   info_vpeq_refl : "\<forall> a u. (a \<sim> u \<sim> a)"
+    and   info_step_def : "step a \<equiv> {(P, Q). (\<Gamma> \<turnstile> P -pes-(actk a)\<rightarrow> Q) \<and> 
                                 ((\<exists>e k. actk a = ((EvtEnt e)\<sharp>k) \<and> eventof a = e 
                                   \<and> dome (gets P)  e = domain a) \<or>
                                   (\<exists>c k. actk a = ((Cmd c)\<sharp>k) \<and> eventof a = (getx P) k 
                                   \<and> dome (gets P) (eventof a) = domain a))}"
-    (*and   step_def : "step a \<equiv> {(P,Q). (P -pes-(actk a)\<rightarrow> Q) \<and> (*domc dome P (actk a)*) 
+    (*and   info_step_def : "step a \<equiv> {(P,Q). (P -pes-(actk a)\<rightarrow> Q) \<and> (*domc dome P (actk a)*) 
                                 dom_helper dome (gets P) (getx P) (Act (actk a)) (K (actk a)) = domain a}"*)
 begin
 
@@ -36,19 +36,16 @@ definition vpeqC :: "('l,'k,'s, 'prog) pesconf \<Rightarrow> 'd \<Rightarrow> ('
    where "vpeqC C1 u C2 \<equiv> (gets C1) \<sim>u\<sim> (gets C2)"
 
 lemma vpeqC_transitive: "\<forall> a b c u. (a \<sim>.u.\<sim> b) \<and> (b \<sim>.u.\<sim> c) \<longrightarrow> (a \<sim>.u.\<sim> c)"
-  using vpeq_transitive vpeqC_def by blast
+  using info_vpeq_trans vpeqC_def by blast
 
 lemma vpeqC_symmetric: "\<forall> a b u. (a \<sim>.u.\<sim> b) \<longrightarrow> (b \<sim>.u.\<sim> a)"
-  using vpeq_symmetric vpeqC_def by blast
+  using info_vpeq_sym vpeqC_def by blast
 
 lemma vpeqC_reflexive: "\<forall> a u. (a \<sim>.u.\<sim> a)"
-  by (simp add: vpeq_reflexive vpeqC_def)
+  by (simp add: info_vpeq_refl vpeqC_def)
 
 definition obsC :: " ('l,'k,'s,'prog) pesconf \<Rightarrow> 'd \<Rightarrow> 'o" (infixl "\<guillemotright>."  55)
   where "C \<guillemotright>. d= (gets C) \<guillemotright> d"
-
-interpretation SM_IFS C0 step domain obsC vpeqC interference
-  using SM_IFS_def vpeqC_reflexive vpeqC_symmetric vpeqC_transitive by blast
 
 definition nextC :: "('l,'k,'s,'prog) pesconf \<Rightarrow> ('l,'k,'s,'prog,'d) action \<Rightarrow>  ('l,'k,'s,'prog) pesconf set" where
   "nextC P a \<equiv> {Q. (P,Q)\<in>step a}"
@@ -63,6 +60,25 @@ definition reachableC :: "('l,'k,'s,'prog) pesconf \<Rightarrow> ('l,'k,'s,'prog
 definition reachableC0 :: "('l,'k,'s,'prog) pesconf \<Rightarrow> bool"  where
   "reachableC0 C \<equiv> reachableC C0 C"
 
+
+subsection \<open>Unwinding Conditions\<close>
+
+definition observed_consistentC :: "bool" where
+ "observed_consistentC \<equiv> (\<forall> s t u. ((s \<sim> u \<sim> t) \<longrightarrow> s \<guillemotright> u  = t \<guillemotright> u))"
+
+definition local_respectC :: "bool" where
+  "local_respectC \<equiv> \<forall>a u C. (reachableC0 C) \<longrightarrow> (\<not> (domain a) \<leadsto> u) \<longrightarrow> 
+                              (\<forall> C'. (C'\<in>nextC C a) \<longrightarrow> (C \<sim>.u.\<sim> C'))"
+
+
+definition weak_step_consistentC :: "bool" where
+  "weak_step_consistentC \<equiv> \<forall>a u C1 C2. (reachableC0 C1) \<and> (reachableC0 C2) \<longrightarrow>  (C1 \<sim>.u.\<sim> C2) 
+                         \<and> ( ((domain a) \<leadsto> u) \<longrightarrow> (C1 \<sim>.(domain a).\<sim> C2) ) \<longrightarrow> 
+                         (\<forall> C1' C2'. (C1'\<in>nextC C1 a) \<and> (C2'\<in>nextC C2 a) \<longrightarrow> (C1' \<sim>.u.\<sim> C2'))"
+
+interpretation SM_IFS C0 step domain obsC vpeqC interference
+  using SM_IFS_def vpeqC_reflexive vpeqC_symmetric vpeqC_transitive by blast
+
 lemma run_equiv : "runC as = run as"
   apply (induct as, simp)
   by (simp add: relcomp_unfold)
@@ -73,22 +89,7 @@ lemma reachableC_equiv : "reachableC C1 C2 = reachable C1 C2"
 lemma reachable0_equiv : "reachableC0 C = reachable0  C"
   by (simp add: reachable0_def reachableC0_def reachableC_equiv)
 
-subsection \<open>Unwinding Conditions\<close>
-
-definition observed_consistentC :: "bool" where
- "observed_consistentC \<equiv> (\<forall> s t u. ((s \<sim> u \<sim> t) \<longrightarrow> s \<guillemotright> u  = t \<guillemotright> u))"
-
-definition local_respectC :: "bool" where
-  "local_respectC \<equiv> \<forall>a u C. (reachableC0 C) \<longrightarrow> ((domain a) \<setminus>\<leadsto> u) \<longrightarrow> 
-                              (\<forall> C'. (C'\<in>nextC C a) \<longrightarrow> (C \<sim>.u.\<sim> C'))"
-
-
-definition weak_step_consistentC :: "bool" where
-  "weak_step_consistentC \<equiv> \<forall>a u C1 C2. (reachableC0 C1) \<and> (reachableC0 C2) \<longrightarrow>  (C1 \<sim>.u.\<sim> C2) 
-                         \<and> ( ((domain a) \<leadsto> u) \<longrightarrow> (C1 \<sim>.(domain a).\<sim> C2) ) \<longrightarrow> 
-                         (\<forall> C1' C2'. (C1'\<in>nextC C1 a) \<and> (C2'\<in>nextC C2 a) \<longrightarrow> (C1' \<sim>.u.\<sim> C2'))"
-
-lemma PiCore_obs_consistent : "observed_consistentC \<Longrightarrow> observed_consistent "
+lemma PiCore_obs_consistent : "observed_consistentC \<Longrightarrow> observed_consistent"
   by (simp add: obsC_def observed_consistentC_def observed_consistent_def vpeqC_def)
 
 lemma local_respectC_equiv : "local_respectC \<longleftrightarrow> local_respect"
@@ -97,8 +98,7 @@ proof
   then show "local_respect"
     apply (simp add: local_respectC_def local_respect_def, clarify)
     apply (drule_tac a = a and b = d and c = aa and d = ab and e = b in all5_imp2D)
-      apply (simp add: reachable0_equiv)
-     apply (simp add:  noninterf_def)
+      apply (simp add: reachable0_equiv, simp)
     by (simp add:  nextC_def)
 next
   assume "local_respect"
@@ -106,7 +106,7 @@ next
     apply (simp add: local_respectC_def local_respect_def, clarify)
     apply (drule_tac a = a and b = u and c = aa and d = ab and e = b in all5_impD)
     using reachable0_equiv apply auto[1]
-    by (simp add: nextC_def noninterf_def)
+    by (simp add: nextC_def)
 qed
 
 lemma weak_step_consistentC_equiv : "weak_step_consistentC \<longleftrightarrow> weak_step_consistent"
